Lean4Lean/Environment.lean
@@ -4,9 +4,10 @@ import Lean4Lean.Inductive.Add
 import Lean4Lean.Primitive
 
 namespace Lean4Lean
-open Lean TypeChecker Environment
+open Lean hiding Environment Exception
+open TypeChecker Kernel Environment
 
-open private add from Lean.Environment
+open private Lean.Kernel.Environment.add from Lean.Environment
 
 def checkConstantVal (env : Environment) (v : ConstantVal) (allowPrimitive := false) : M Unit := do
   checkName env v.name allowPrimitive
@@ -16,20 +17,20 @@ def checkConstantVal (env : Environment) (v : ConstantVal) (allowPrimitive := fa
   _ ← ensureSort sort v.type
 
 def addAxiom (env : Environment) (v : AxiomVal) (check := true) :
-    Except KernelException Environment := do
+    Except Exception Environment := do
   if check then
     _ ← (checkConstantVal env v.toConstantVal).run env
       (safety := if v.isUnsafe then .unsafe else .safe)
-  return add env (.axiomInfo v)
+  return env.add (.axiomInfo v)
 
 def addDefinition (env : Environment) (v : DefinitionVal) (check := true) :
-    Except KernelException Environment := do
+    Except Exception Environment := do
   if let .unsafe := v.safety then
     -- Meta definition can be recursive.
     -- So, we check the header, add, and then type check the body.
     if check then
       _ ← (checkConstantVal env v.toConstantVal).run env (safety := .unsafe)
-    let env' := add env (.defnInfo v)
+    let env' := env.add (.defnInfo v)
     if check then
       checkNoMVarNoFVar env' v.name v.value
       M.run env' (safety := .unsafe) (lctx := {}) do
@@ -45,10 +46,10 @@ def addDefinition (env : Environment) (v : DefinitionVal) (check := true) :
         let valType ← TypeChecker.check v.value v.levelParams
         if !(← isDefEq valType v.type) then
           throw <| .declTypeMismatch env (.defnDecl v) valType
-    return add env (.defnInfo v)
+    return env.add (.defnInfo v)
 
 def addTheorem (env : Environment) (v : TheoremVal) (check := true) :
-    Except KernelException Environment := do
+    Except Exception Environment := do
   if check then
     -- TODO(Leo): we must add support for handling tasks here
     M.run env (safety := .safe) (lctx := {}) do
@@ -59,20 +60,20 @@ def addTheorem (env : Environment) (v : TheoremVal) (check := true) :
       let valType ← TypeChecker.check v.value v.levelParams
       if !(← isDefEq valType v.type) then
         throw <| .declTypeMismatch env (.thmDecl v) valType
-  return add env (.thmInfo v)
+  return env.add (.thmInfo v)
 
 def addOpaque (env : Environment) (v : OpaqueVal) (check := true) :
-    Except KernelException Environment := do
+    Except Exception Environment := do
   if check then
     M.run env (safety := .safe) (lctx := {}) do
       checkConstantVal env v.toConstantVal
       let valType ← TypeChecker.check v.value v.levelParams
       if !(← isDefEq valType v.type) then
         throw <| .declTypeMismatch env (.opaqueDecl v) valType
-  return add env (.opaqueInfo v)
+  return env.add (.opaqueInfo v)
 
 def addMutual (env : Environment) (vs : List DefinitionVal) (check := true) :
-    Except KernelException Environment := do
+    Except Exception Environment := do
   let v₀ :: _ := vs | throw <| .other "invalid empty mutual definition"
   if let .safe := v₀.safety then
     throw <| .other "invalid mutual definition, declaration is not tagged as unsafe/partial"
@@ -85,7 +86,7 @@ def addMutual (env : Environment) (vs : List DefinitionVal) (check := true) :
         checkConstantVal env v.toConstantVal
   let mut env' := env
   for v in vs do
-    env' := add env' (.defnInfo v)
+    env' := env'.add (.defnInfo v)
   if check then
     M.run env' (safety := v₀.safety) (lctx := {}) do
       for v in vs do
@@ -97,7 +98,7 @@ def addMutual (env : Environment) (vs : List DefinitionVal) (check := true) :
 
 /-- Type check given declaration and add it to the environment -/
 def addDecl (env : Environment) (decl : Declaration) (check := true) :
-    Except KernelException Environment := do
+    Except Exception Environment := do
   match decl with
   | .axiomDecl v => addAxiom env v check
   | .defnDecl v => addDefinition env v check
