Lean4Lean/Environment/Basic.lean
@@ -1,13 +1,16 @@
 import Lean.Environment
 
-namespace Lean.Environment
+namespace Lean.Kernel.Environment
 
-def get (env : Environment) (n : Name) : Except KernelException ConstantInfo :=
+def contains (env : Environment) (n : Name) : Bool :=
+  env.constants.contains n
+
+def get (env : Environment) (n : Name) : Except Exception ConstantInfo :=
   match env.find? n with
   | some ci => pure ci
   | none => throw <| .unknownConstant env n
 
-def checkDuplicatedUnivParams : List Name → Except KernelException Unit
+def checkDuplicatedUnivParams : List Name → Except Exception Unit
   | [] => pure ()
   | p :: ls => do
     if p ∈ ls then
@@ -15,15 +18,15 @@ def checkDuplicatedUnivParams : List Name → Except KernelException Unit
         s!"failed to add declaration to environment, duplicate universe level parameter: '{p}'"
     checkDuplicatedUnivParams ls
 
-def checkNoMVar (env : Environment) (n : Name) (e : Expr) : Except KernelException Unit := do
+def checkNoMVar (env : Environment) (n : Name) (e : Expr) : Except Exception Unit := do
   if e.hasMVar then
     throw <| .declHasMVars env n e
 
-def checkNoFVar (env : Environment) (n : Name) (e : Expr) : Except KernelException Unit := do
+def checkNoFVar (env : Environment) (n : Name) (e : Expr) : Except Exception Unit := do
   if e.hasFVar then
     throw <| .declHasFVars env n e
 
-def checkNoMVarNoFVar (env : Environment) (n : Name) (e : Expr) : Except KernelException Unit := do
+def checkNoMVarNoFVar (env : Environment) (n : Name) (e : Expr) : Except Exception Unit := do
   checkNoMVar env n e
   checkNoFVar env n e
 
@@ -34,8 +37,18 @@ def primitives : NameSet := .ofList [
   ``Nat.gcd, ``Nat.mod, ``Nat.div, ``Nat.beq, ``Nat.ble,
   ``String, ``String.mk]
 
+/--
+Returns true iff `constName` is a non-recursive inductive datatype that has only one constructor and no indices.
+
+Such types have special kernel support. This must be in sync with `is_structure_like`.
+-/
+def isStructureLike (env : Environment) (constName : Name) : Bool :=
+  match env.find? constName with
+  | some (.inductInfo { isRec := false, ctors := [_], numIndices := 0, .. }) => true
+  | _ => false
+
 def checkName (env : Environment) (n : Name)
-    (allowPrimitive := false) : Except KernelException Unit := do
+    (allowPrimitive := false) : Except Exception Unit := do
   if env.contains n then
     throw <| .alreadyDeclared env n
   unless allowPrimitive do
