Lean4Lean/Quot.lean
@@ -5,9 +5,10 @@ import Lean4Lean.Instantiate
 import Lean4Lean.LocalContext
 
 namespace Lean4Lean
-open Lean
+open Lean hiding Environment Exception
+open Kernel
 
-open private add markQuotInit from Lean.Environment
+open private Lean.Kernel.Environment.add markQuotInit from Lean.Environment
 
 abbrev ExprBuildT (m) := ReaderT LocalContext <| ReaderT NameGenerator m
 
@@ -16,8 +17,8 @@ def ExprBuildT.run [Monad m] (x : ExprBuildT m α) : m α := x {} {}
 instance : MonadLocalNameGenerator (ExprBuildT m) where
   withFreshId x c ngen := x ngen.curr c ngen.next
 
-def checkEqType (env : Environment) : Except KernelException Unit := do
-  let fail {α} (s : String) : Except KernelException α :=
+def checkEqType (env : Environment) : Except Exception Unit := do
+  let fail {α} (s : String) : Except Exception α :=
     throw <| .other s!"failed to initialize quot module, {s}"
   let .inductInfo info ← env.get ``Eq | fail "environment does not have 'Eq' type"
   let [u] := info.levelParams | fail "unexpected number of universe params at 'Eq' type"
@@ -34,21 +35,21 @@ def checkEqType (env : Environment) : Except KernelException Unit := do
         if info.type != ((← read).mkForall' #[α, a] <| mkApp3 (.const ``Eq [.param u]) α a a) then
           fail "unexpected type for 'Eq' type constructor"
 
-def Environment.addQuot (env : Environment) : Except KernelException Environment := do
-  if env.header.quotInit then return env
+def Environment.addQuot (env : Environment) : Except Exception Environment := do
+  if env.quotInit then return env
   checkEqType env
   ExprBuildT.run do
   let u := .param `u
   withLocalDecl `α (.sort u) .implicit fun α => do
   let env ← withLocalDecl `r (.arrow α (.arrow α .prop)) .default fun r => do
     -- constant Quot.{u} {α : Sort u} (r : α → α → Prop) : Sort u
-    let env := add env <| .quotInfo {
+    let env := env.add <| .quotInfo {
       name := ``Quot, kind := .type, levelParams := [`u]
       type := (← read).mkForall' #[α, r] <| .sort u
     }
     withLocalDecl `a α .default fun a => do
       -- constant Quot.mk.{u} {α : Sort u} (r : α → α → Prop) (a : α) : @Quot.{u} α r
-      return add env <| .quotInfo {
+      return env.add <| .quotInfo {
         name := ``Quot.mk, kind := .ctor, levelParams := [`u]
         type := (← read).mkForall' #[α, r, a] <| mkApp2 (.const ``Quot [u]) α r
       }
@@ -64,7 +65,7 @@ def Environment.addQuot (env : Environment) : Except KernelException Environment
     let sanity := (← read).mkForall' #[a, b] <| .arrow rab fa_eq_fb
     -- constant Quot.lift.{u, v} {α : Sort u} {r : α → α → Prop} {β : Sort v} (f : α → β) :
     --   (∀ a b : α, r a b → f a = f b) → @Quot.{u} α r → β
-    return add env <| .quotInfo {
+    return env.add <| .quotInfo {
       name := ``Quot.lift, kind := .lift, levelParams := [`u, `v]
       type := (← read).mkForall' #[α, r, β, f] <| .arrow sanity <| .arrow quot_r β
     }
@@ -74,7 +75,7 @@ def Environment.addQuot (env : Environment) : Except KernelException Environment
   withLocalDecl `q quot_r .implicit fun q => do
   -- constant Quot.ind.{u} {α : Sort u} {r : α → α → Prop} {β : @Quot.{u} α r → Prop} :
   --   (∀ a : α, β (@Quot.mk.{u} α r a)) → ∀ q : @Quot.{u} α r, β q */
-  let env := add env <| .quotInfo {
+  let env := env.add <| .quotInfo {
     name := ``Quot.ind, kind := .ind, levelParams := [`u]
     type := (← read).mkForall' #[α, r, β] <|
       .forallE `mk all_quot ((← read).mkForall' #[q] <| .app β q) .default
